isabelle-thys/Programs.thy
@@ -233,7 +233,7 @@ valid_oracle_program_Seq:  \<open>valid_oracle_program c \<Longrightarrow> valid
 | valid_oracle_program_Sample: \<open>(\<And>m. weight (e m) \<le> 1) \<Longrightarrow> valid_oracle_program (Sample e)\<close>
 | valid_oracle_program_IfThenElse: \<open>valid_oracle_program c \<Longrightarrow> valid_oracle_program d \<Longrightarrow> valid_oracle_program (IfThenElse e c d)\<close>
 | valid_oracle_program_While: \<open>valid_oracle_program c \<Longrightarrow> valid_oracle_program (While e c)\<close>
-| valid_oracle_program_QuantumOp: \<open>(\<And>m. km_norm (e m) \<le> 1) \<Longrightarrow> valid_oracle_program (QuantumOp e)\<close>
+| valid_oracle_program_QuantumOp: \<open>(\<And>m. kraus_map (e m)) \<Longrightarrow> (\<And>m. km_norm (e m) \<le> 1) \<Longrightarrow> valid_oracle_program (QuantumOp e)\<close>
 | valid_oracle_program_Measurement: \<open>valid_oracle_program (Measurement e)\<close>
 | valid_oracle_program_InstantiateOracles: \<open>(\<And>d. d \<in> set ds \<Longrightarrow> valid_oracle_program d \<and> no_oracles d) \<Longrightarrow> valid_oracle_program c \<Longrightarrow> 
   oracle_number c \<le> length ds \<Longrightarrow> valid_oracle_program (InstantiateOracles c ds)\<close>
@@ -422,7 +422,7 @@ fun block :: \<open>program list \<Rightarrow> program\<close> where
 | block_cons[simp del]: \<open>block (p#ps) = seq p (block ps)\<close>
 
 lift_definition sample :: \<open>'a cvariable \<Rightarrow> 'a distr expression \<Rightarrow> program\<close> is
-  \<open>\<lambda>X e. Sample (\<lambda>m::cl. map_distr (\<lambda>x. setter X x m) (e m))\<close>
+  \<open>\<lambda>X e. Sample (\<lambda>m::cl. map_distr (\<lambda>x. Classical_Registers.setter X x m) (e m))\<close>
   by (simp add: valid_oracle_program.intros no_oracles.intros valid_program_def)
 
 definition assign :: \<open>'a cvariable \<Rightarrow> 'a expression \<Rightarrow> program\<close> where
@@ -633,6 +633,8 @@ proof (rule continuous_on_compose2[OF _ assms])
   show \<open>f ` X \<subseteq> UNIV\<close>
     by simp
   define S where \<open>S = range apply_denotation\<close>
+  have S_def': \<open>S = Collect (is_cq_map qFst)\<close>
+    using S_def type_definition.Rep_range type_definition_denotation by blast
   have \<open>openin (top_of_set UNIV) (UNIV \<inter> apply_denotation -` U) \<longleftrightarrow> openin (top_of_set S) U\<close> if \<open>U \<subseteq> S\<close> for U
   proof -
     define RU where \<open>RU = apply_denotation -` U\<close>
@@ -641,7 +643,7 @@ proof (rule continuous_on_compose2[OF _ assms])
     have \<open>openin (top_of_set UNIV) (UNIV \<inter> RU) = open RU\<close>
       by (simp add: openin_subtopology)
     also have \<open>\<dots> = (\<exists>T. open T \<and> U = T \<inter> S)\<close>
-      by (simp add: open_denotation_def openin_subtopology S_def U_def)
+      by (simp add: open_denotation_def openin_subtopology S_def' U_def)
     also have \<open>\<dots> = openin (top_of_set S) U\<close>
       by (simp add: openin_subtopology)
     finally show ?thesis
@@ -651,6 +653,40 @@ proof (rule continuous_on_compose2[OF _ assms])
     apply (rule_tac quotient_map_imp_continuous_open[where T=S])
     using apply_denotation by (auto simp: S_def)
 qed
+
+(* lemma continuous_on_Abs_denotation[continuous_intros]:
+  assumes \<open>continuous_on X f\<close>
+  shows \<open>continuous_on X (\<lambda>x. Abs_denotation (f x))\<close>
+proof (rule continuous_on_compose2[OF _ assms  order_refl])
+  define S where \<open>S = Abs_denotation ` f ` X\<close>
+  have \<open>openin (top_of_set (f ` X)) ((f ` X) \<inter> Abs_denotation -` U) \<longleftrightarrow> openin (top_of_set S) U\<close> if \<open>U \<subseteq> S\<close> for U
+  proof -
+    define RU where \<open>RU = Abs_denotation -` U\<close>
+    have U_def: \<open>U = Abs_denotation ` RU\<close>
+      using RU_def S_def that by blast
+    have \<open>openin (top_of_set (f ` X)) ((f ` X) \<inter> RU) = open RU\<close>
+try0
+sledgehammer [dont_slice]
+by -
+
+      by (simp add: openin_subtopology)
+    also have \<open>\<dots> = (\<exists>T. open T \<and> U = T \<inter> S)\<close>
+      apply (simp add: open_denotation_def openin_subtopology S_def U_def)
+
+try0
+sledgehammer [dont_slice]
+by -
+
+    also have \<open>\<dots> = openin (top_of_set S) U\<close>
+      by (simp add: openin_subtopology)
+    finally show ?thesis
+      by (simp add: RU_def)
+  qed
+  then show \<open>continuous_on (f ` X) Abs_denotation\<close>
+    apply (rule_tac quotient_map_imp_continuous_open[where T=S])
+    using apply_denotation by (auto simp: S_def)
+qed *)
+
 
 instance denotation :: pospace
 proof (rule pospaceI)
@@ -688,43 +724,391 @@ lemma infsum_le_finite_sums:
   by (metis has_sum_le_finite_sums assms bot_least finite.intros(1) has_sum_infsum infsum_not_exists
       sum.empty)
 
+(* TODO move *)
+lemma kraus_map_sum:
+  assumes \<open>\<And>x. x\<in>A \<Longrightarrow> kraus_map (\<EE> x)\<close>
+  shows \<open>kraus_map (\<Sum>x\<in>A. \<EE> x)\<close>
+  apply (insert assms, induction A rule:infinite_finite_induct)
+  by auto
+
+(* TODO move *)
+lemma km_bound_sum:
+  assumes \<open>\<And>x. x\<in>A \<Longrightarrow> kraus_map (\<EE> x)\<close>
+  shows \<open>km_bound (\<Sum>x\<in>A. \<EE> x) = (\<Sum>x\<in>A. km_bound (\<EE> x))\<close>
+proof (insert assms, induction A rule:infinite_finite_induct)
+  case (infinite A)
+  then show ?case
+    by (metis km_bound_0 sum.infinite)
+next
+  case empty
+  then show ?case
+    by (metis km_bound_0 sum.empty)
+next
+  case (insert x F)
+  have \<open>km_bound (\<Sum>x\<in>insert x F. \<EE> x) = km_bound (\<EE> x + (\<Sum>x\<in>F. \<EE> x))\<close>
+    by (simp add: insert.hyps)
+  also have \<open>\<dots> = km_bound (\<EE> x) + km_bound (\<Sum>x\<in>F. \<EE> x)\<close>
+    by (simp add: km_bound_plus kraus_map_sum insert.prems)
+  also have \<open>\<dots> = km_bound (\<EE> x) + (\<Sum>x\<in>F. km_bound (\<EE> x))\<close>
+    by (simp add: insert)
+  also have \<open>\<dots> = (\<Sum>x\<in>insert x F. km_bound (\<EE> x))\<close>
+    using insert.hyps by fastforce
+  finally show ?case
+    by -
+qed
+
+
+(* TODO move *)
+lemma apply_denotation_sum: \<open>apply_denotation (\<Sum>x\<in>A. \<EE> x) = (\<Sum>x\<in>A. apply_denotation (\<EE> x))\<close>
+proof (induction A rule:infinite_finite_induct)
+  case (infinite A)
+  then show ?case
+    by simp
+next
+  case empty
+  then show ?case
+    by simp
+next
+  case (insert x F)
+  have \<open>apply_denotation (\<Sum>x\<in>insert x F. \<EE> x) = apply_denotation (\<EE> x + (\<Sum>x\<in>F. \<EE> x))\<close>
+    by (simp add: insert.hyps)
+  also have \<open>\<dots> = apply_denotation (\<EE> x) + apply_denotation (\<Sum>x\<in>F. \<EE> x)\<close>
+    by (auto simp: plus_denotation.rep_eq)
+  also have \<open>\<dots> = apply_denotation (\<EE> x) + (\<Sum>x\<in>F. apply_denotation (\<EE> x))\<close>
+    by (simp add: insert)
+  also have \<open>\<dots> = (\<Sum>x\<in>insert x F. apply_denotation (\<EE> x))\<close>
+    using insert.hyps by fastforce
+  finally show ?case
+    by -
+qed
+
+(* lemma [transfer_rule]:
+  includes lifting_syntax
+  shows \<open>(rel_set (rel_filter cr_denotation) ===> rel_filter cr_denotation) Inf Inf\<close>
+  unfolding Inf_filter_def
+  apply transfer_prover_start
+
+  apply transfer_step
+  apply transfer_step
+  apply transfer_step
+   apply transfer_step
+  apply (auto intro!: simp: )
+  apply (subst Domainp_rel_filter)
+   apply (subst denotation.domain)
+apply (simp add: )
+ *)
+
+(* lemma [transfer_rule]:
+  includes lifting_syntax
+  shows \<open>(cr_denotation ===> rel_filter cr_denotation) nhds nhds\<close>
+  unfolding nhds_def
+  apply transfer_prover_start
+  apply transfer_step
+  apply transfer_step
+  apply transfer_step
+  apply transfer_step
+  apply transfer_step
+  apply transfer_step
+  apply transfer_step *)
+
+
+lemma in_range_image_iff: \<open>V \<in> range ((`) f) \<longleftrightarrow> V \<subseteq> range f\<close>
+  by force
+
+
+lemma tendsto_denotation_apply_denotation:
+  \<open>(g \<longlongrightarrow> t) F \<longleftrightarrow> ((\<lambda>x. apply_denotation (g x)) \<longlongrightarrow> apply_denotation t) F\<close>
+proof -
+  define s f where \<open>s = apply_denotation t\<close> and \<open>f x = apply_denotation (g x)\<close> for x
+  define T :: \<open>(((cl \<times> qu) ell2, _) trace_class \<Rightarrow> _) topology\<close>
+    where \<open>T = top_of_set (Collect (is_cq_map qFst))\<close>
+
+  have [simp]: \<open>apply_denotation x \<in> apply_denotation ` U \<longleftrightarrow> x \<in> U\<close> for x U
+    using apply_denotation_inject by fastforce
+  have [iff]: \<open>apply_denotation t \<in> topspace T\<close>
+    using T_def apply_denotation by force
+  have app_den_cq_map: \<open>V \<in> range (image apply_denotation) \<longleftrightarrow> V \<subseteq> Collect (is_cq_map qFst)\<close> for V
+    apply (simp add: in_range_image_iff flip: Ball_Collect)
+    by (smt (verit, ccfv_threshold) Abs_denotation_inverse apply_denotation imageE mem_Collect_eq rangeI subsetI
+        subset_image_iff)
+  have \<open>(g \<longlongrightarrow> t) F \<longleftrightarrow> (\<forall>U. open U \<longrightarrow> t \<in> U \<longrightarrow> (\<forall>\<^sub>F x in F. g x \<in> U))\<close>
+    by (simp add: limitin_def flip: limitin_canonical_iff)
+  also have \<open>\<dots> \<longleftrightarrow> (\<forall>U. openin T (apply_denotation ` U) \<longrightarrow> t \<in> U \<longrightarrow> (\<forall>\<^sub>F x in F. g x \<in> U))\<close>
+    using T_def open_denotation.rep_eq by presburger
+  also have \<open>\<dots> \<longleftrightarrow> (\<forall>U. openin T (apply_denotation ` U) \<longrightarrow> s \<in> apply_denotation ` U \<longrightarrow> (\<forall>\<^sub>F x in F. f x \<in> apply_denotation ` U))\<close>
+    by (simp add: f_def s_def)
+  also have \<open>\<dots> \<longleftrightarrow> (\<forall>V\<in>range (image apply_denotation). openin T V \<longrightarrow> s \<in> V \<longrightarrow> (\<forall>\<^sub>F x in F. f x \<in> V))\<close>
+    by blast
+  also have \<open>\<dots> \<longleftrightarrow> (\<forall>V\<subseteq>Collect (is_cq_map qFst). openin T V \<longrightarrow> s \<in> V \<longrightarrow> (\<forall>\<^sub>F x in F. f x \<in> V))\<close>
+    by (simp add: app_den_cq_map Ball_def)
+  also have \<open>\<dots> \<longleftrightarrow> (\<forall>V. openin T V \<longrightarrow> s \<in> V \<longrightarrow> (\<forall>\<^sub>F x in F. f x \<in> V))\<close>
+    apply (rule all_cong1)
+    by (auto simp: T_def openin_open)
+  also have \<open>\<dots> \<longleftrightarrow> limitin T f s F\<close>
+    by (simp add: limitin_def s_def)
+  also have \<open>\<dots> \<longleftrightarrow> (f \<longlongrightarrow> s) F\<close>
+    using apply_denotation by (simp add: T_def limitin_subtopology s_def f_def)
+  finally show \<open>(g \<longlongrightarrow> t) F \<longleftrightarrow> (f \<longlongrightarrow> s) F\<close>
+    by -
+qed
+
+lemma tendsto_denotation_transfer[transfer_rule]:
+  includes lifting_syntax
+  shows \<open>(((=) ===> cr_denotation) ===> cr_denotation ===> (=) ===> (\<longleftrightarrow>))
+           tendsto tendsto\<close>
+proof (intro rel_funI, rename_tac f g s t F G)
+  fix g :: \<open>'c \<Rightarrow> denotation\<close> and f s t and F G :: \<open>'c filter\<close>
+  assume \<open>((=) ===> cr_denotation) f g\<close> and st: \<open>cr_denotation s t\<close> and [symmetric, simp]: \<open>F = G\<close>
+  then have fg: \<open>cr_denotation (f x) (g x)\<close> for x
+    by (simp add: rel_fun_def)
+  from st have st': \<open>s = apply_denotation t\<close>
+    by (meson cr_denotation_def)
+  from fg have fg': \<open>f x = apply_denotation (g x)\<close> for x
+    by (simp add: cr_denotation_def)
+  show \<open>(f \<longlongrightarrow> s) F \<longleftrightarrow> (g \<longlongrightarrow> t) G\<close>
+    by (simp add: st' fg'[abs_def] tendsto_denotation_apply_denotation)
+qed
+
+lemma has_sum_denotation_apply_denotation:
+  \<open>(g has_sum t) A \<longleftrightarrow> ((\<lambda>x. apply_denotation (g x)) has_sum apply_denotation t) A\<close>
+proof -
+  have \<open>(g has_sum t) A \<longleftrightarrow> (sum g \<longlongrightarrow> t) (finite_subsets_at_top A)\<close>
+    by (simp add: has_sum_def)
+  also have \<open>\<dots> \<longleftrightarrow> ((\<lambda>F. apply_denotation (\<Sum>x\<in>F. g x)) \<longlongrightarrow> apply_denotation t) (finite_subsets_at_top A)\<close>
+    by (simp add: tendsto_denotation_apply_denotation)
+  also have \<open>\<dots> \<longleftrightarrow> ((\<lambda>F. \<Sum>x\<in>F. apply_denotation (g x)) \<longlongrightarrow> apply_denotation t) (finite_subsets_at_top A)\<close>
+    by (simp add: apply_denotation_sum)
+  also have \<open>\<dots> \<longleftrightarrow> ((\<lambda>x. apply_denotation (g x)) has_sum apply_denotation t) A\<close>
+    by (simp add: has_sum_def)
+  finally show ?thesis
+    by -
+qed
+
+lemma has_sum_denotation_transfer[transfer_rule]:
+  includes lifting_syntax
+  shows \<open>(((=) ===> cr_denotation) ===> (=) ===> cr_denotation ===> (\<longleftrightarrow>)) HAS_SUM HAS_SUM\<close>
+proof (intro rel_funI, rename_tac f g A B s t)
+  fix g :: \<open>'a \<Rightarrow> denotation\<close> and f s t and A B :: \<open>'a set\<close>
+  assume \<open>((=) ===> cr_denotation) f g\<close> and st: \<open>cr_denotation s t\<close> and [symmetric, simp]: \<open>A = B\<close>
+  then have fg: \<open>cr_denotation (f x) (g x)\<close> for x
+    by (simp add: rel_fun_def)
+  from st have st': \<open>s = apply_denotation t\<close>
+    by (meson cr_denotation_def)
+  from fg have fg': \<open>f x = apply_denotation (g x)\<close> for x
+    by (simp add: cr_denotation_def)
+  show \<open>(f has_sum s) A \<longleftrightarrow> (g has_sum t) B\<close>
+    by (simp add: st' fg'[abs_def] has_sum_denotation_apply_denotation)
+qed
+
+lemma has_sum_coordinatewise:
+  \<open>(f has_sum s) A \<longleftrightarrow> (\<forall>i. ((\<lambda>x. f x i) has_sum s i) A)\<close>
+proof -
+  have \<open>(f has_sum s) A \<longleftrightarrow> ((\<lambda>F. (\<Sum>x\<in>F. f x)) \<longlongrightarrow> s) (finite_subsets_at_top A)\<close>
+    by (simp add: has_sum_def)
+  also  have \<open>\<dots> \<longleftrightarrow> (\<forall>i. ((\<lambda>F. (\<Sum>x\<in>F. f x) i) \<longlongrightarrow> s i) (finite_subsets_at_top A))\<close>
+    by (simp add: tendsto_coordinatewise)
+  also have \<open>\<dots> \<longleftrightarrow> (\<forall>i. ((\<lambda>F. \<Sum>x\<in>F. f x i) \<longlongrightarrow> s i) (finite_subsets_at_top A))\<close>
+  proof (rewrite at \<open>\<Sum>x\<in>F. f x i\<close> at \<open>\<lambda>F. \<hole>\<close> in \<open>\<forall>i. \<hole>\<close> to \<open>(\<Sum>x\<in>F. f x) i\<close> DEADID.rel_mono_strong)
+    fix i
+    show \<open>(\<Sum>x\<in>F. f x i) = (\<Sum>x\<in>F. f x) i\<close> for F
+      apply (induction F rule:infinite_finite_induct)
+      by auto
+    show \<open>P = P\<close> for P :: bool
+      by simp
+  qed
+  also have \<open>\<dots> \<longleftrightarrow> (\<forall>i. ((\<lambda>x. f x i) has_sum s i) A)\<close>
+    by (simp add: has_sum_def)
+  finally show ?thesis
+    by - 
+qed
+
+
+lemma is_cq_map_tendsto:
+  assumes cq: \<open>\<forall>\<^sub>F x in F. is_cq_map Q (\<EE> x)\<close>
+  assumes nontrivial: \<open>F \<noteq> \<bottom>\<close>
+  assumes \<EE>lim: \<open>(\<EE> \<longlongrightarrow> \<FF>) F\<close>
+  assumes kraus: \<open>kraus_map \<FF>\<close>
+  shows \<open>is_cq_map Q \<FF>\<close>
+proof -
+  have \<open>(cq_id Q o \<FF> o cq_id Q) = \<FF>\<close>
+  proof (rule ext)
+    fix t :: \<open>('c ell2, 'c ell2) trace_class\<close>
+    have cont: \<open>continuous_on UNIV (\<lambda>a. cq_id Q \<circ> a \<circ> cq_id Q)\<close>
+      by (auto intro!: continuous_intros)
+    from \<open>(\<EE> \<longlongrightarrow> \<FF>) F\<close>
+    have \<open>((\<lambda>x. cq_id Q o (\<EE> x) o cq_id Q) \<longlongrightarrow> cq_id Q o \<FF> o cq_id Q) F\<close>
+      apply (rule tendsto_compose_at_within[unfolded o_def, where S=UNIV])
+      using cont
+      by (auto simp: o_def continuous_on_def)
+    then have \<open>(\<EE> \<longlongrightarrow> cq_id Q o \<FF> o cq_id Q) F\<close>
+      apply (rule tendsto_cong[THEN iffD1, rotated])
+      using cq unfolding is_cq_map_def
+      apply (rule eventually_mono)
+      by simp
+    then have 1: \<open>((\<lambda>x. \<EE> x t) \<longlongrightarrow> (cq_id Q o \<FF> o cq_id Q) t) F\<close>
+      by (simp add: tendsto_coordinatewise)
+    from \<open>(\<EE> \<longlongrightarrow> \<FF>) F\<close>
+    have 2: \<open>((\<lambda>x. \<EE> x t) \<longlongrightarrow> \<FF> t) F\<close>
+      by (simp add: tendsto_coordinatewise)
+    from nontrivial 1 2 show \<open>(cq_id Q o \<FF> o cq_id Q) t = \<FF> t\<close>
+      by (rule tendsto_unique)
+  qed
+  with kraus
+  show \<open>is_cq_map Q \<FF>\<close>
+    using is_cq_map_def by blast
+qed
+
+term \<open>kf_summable \<EE> A \<longleftrightarrow> summable_on_in cweak_operator_topology (\<lambda>a. kf_bound (\<EE> a)) A\<close>
+term \<open>trace_tc (\<EE> *\<^sub>k\<^sub>r \<rho>) = trace_tc (compose_tcr (kf_bound \<EE>) \<rho>)\<close>
+term \<open>\<psi> \<bullet>\<^sub>C kf_bound \<EE> \<phi> = trace_tc (\<EE> *\<^sub>k\<^sub>r tc_butterfly \<phi> \<psi>)\<close>
+
+lemma kraus_map_has_sum:
+  assumes \<open>\<And>x. x \<in> A \<Longrightarrow> kraus_map (\<EE> x)\<close>
+  assumes \<open>km_summable \<EE> A\<close>
+  assumes \<open>(\<EE> has_sum \<FF>) A\<close>
+  shows \<open>kraus_map \<FF>\<close>
+proof -
+  from \<open>(\<EE> has_sum \<FF>) A\<close>
+  have \<open>((\<lambda>x. \<EE> x t) has_sum \<FF> t) A\<close> for t
+    by (simp add: has_sum_coordinatewise)
+  then have \<open>\<FF> t = (\<Sum>\<^sub>\<infinity>a\<in>A. \<EE> a t)\<close> for t
+    by (metis infsumI)
+  with kraus_map_infsum[OF assms(1,2)]
+  show \<open>kraus_map \<FF>\<close>
+    by presburger
+qed
+
+
+lemma is_cq_map_sum:
+  assumes cq: \<open>\<And>x. x \<in> A \<Longrightarrow> is_cq_map Q (\<EE> x)\<close>
+  shows \<open>is_cq_map Q (\<Sum>x\<in>A. \<EE> x)\<close>
+  using cq apply (induction A rule:infinite_finite_induct)
+  by (auto simp: is_cq_map_0 func_plus is_cq_map_plus simp flip: zero_fun_apply)
+
+lemma is_cq_map_has_sum:
+  assumes cq: \<open>\<And>x. x \<in> A \<Longrightarrow> is_cq_map Q (\<EE> x)\<close>
+  assumes \<EE>summable: \<open>km_summable \<EE> A\<close>
+  assumes \<EE>sum: \<open>(\<EE> has_sum \<FF>) A\<close>
+  shows \<open>is_cq_map Q \<FF>\<close>
+proof -
+  from \<EE>summable \<EE>sum
+  have \<open>kraus_map \<FF>\<close>
+    apply (rule kraus_map_has_sum[rotated])
+    using cq is_cq_map_def by blast
+  from \<EE>sum
+  have \<open>(sum \<EE> \<longlongrightarrow> \<FF>) (finite_subsets_at_top A)\<close>
+    by (simp add: has_sum_def)
+  then show \<open>is_cq_map Q \<FF>\<close>
+    apply (rule is_cq_map_tendsto[rotated 2])
+    using \<open>kraus_map \<FF>\<close> assms
+    by (auto intro!: eventually_finite_subsets_at_top_weakI is_cq_map_sum)
+qed
+
+lemma km_summable_iff_sums_to_kraus_map:
+  assumes \<open>\<And>a. a\<in>A \<Longrightarrow> kraus_map (\<EE> a)\<close>
+  shows \<open>km_summable \<EE> A \<longleftrightarrow> (\<exists>\<FF>. (\<forall>t. ((\<lambda>x. \<EE> x t) has_sum \<FF> t) A) \<and> kraus_map \<FF>)\<close>
+proof (rule iffI)
+  assume asm: \<open>km_summable \<EE> A\<close>
+  define \<FF> where \<open>\<FF> t = (\<Sum>\<^sub>\<infinity>a\<in>A. \<EE> a t)\<close> for t
+  from km_summable_summable[OF assms asm]
+  have \<open>((\<lambda>x. \<EE> x t) has_sum \<FF> t) A\<close> for t
+    using \<FF>_def by fastforce
+  moreover from kraus_map_infsum[OF assms asm]
+  have \<open>kraus_map \<FF>\<close>
+    by (simp add: \<FF>_def[abs_def])
+  ultimately show \<open>(\<exists>\<FF>. (\<forall>t. ((\<lambda>x. \<EE> x t) has_sum \<FF> t) A) \<and> kraus_map \<FF>)\<close>
+    by auto
+next
+  assume \<open>\<exists>\<FF>. (\<forall>t. ((\<lambda>x. \<EE> x t) has_sum \<FF> t) A) \<and> kraus_map \<FF>\<close>
+  then obtain \<FF> where \<open>kraus_map \<FF>\<close> and \<open>((\<lambda>x. \<EE> x t) has_sum \<FF> t) A\<close> for t
+    by auto
+  then have \<open>((\<lambda>x. trace_tc (\<EE> x (tc_butterfly k h))) has_sum trace_tc (\<FF> (tc_butterfly k h))) A\<close> for h k
+    using bounded_clinear.bounded_linear bounded_clinear_trace_tc has_sum_bounded_linear by blast
+  then have \<open>((\<lambda>x. trace_tc (\<EE> x (tc_butterfly k h))) has_sum h \<bullet>\<^sub>C (km_bound \<FF> *\<^sub>V k)) A\<close> for h k
+    by (simp add: km_bound_from_map \<open>kraus_map \<FF>\<close>)
+  then have \<open>((\<lambda>x. h \<bullet>\<^sub>C (km_bound (\<EE> x) *\<^sub>V k)) has_sum h \<bullet>\<^sub>C (km_bound \<FF> *\<^sub>V k)) A\<close> for h k
+    apply (rule has_sum_cong[THEN iffD1, rotated 1])
+    by (simp add: km_bound_from_map assms)
+  then have \<open>has_sum_in cweak_operator_topology (\<lambda>a. km_bound (\<EE> a)) A (km_bound \<FF>)\<close>
+    by (simp add: has_sum_in_cweak_operator_topology_pointwise)
+  then show \<open>km_summable \<EE> A\<close>
+    using  summable_on_in_def km_summable_def by blast
+qed
+
+
+lemma summable_on_denotation_apply_denotation:
+  \<open>g summable_on A \<longleftrightarrow> km_summable (\<lambda>x. apply_denotation (g x)) A\<close>
+proof (rule iffI)
+  assume \<open>g summable_on A\<close>
+  then obtain s where \<open>(g has_sum s) A\<close>
+    using summable_on_def by blast
+  define g' s' where \<open>g' x = apply_denotation (g x)\<close> and \<open>s' = apply_denotation s\<close> for x
+  from \<open>(g has_sum s) A\<close>
+  have \<open>(g' has_sum s') A\<close>
+    by (simp add: has_sum_denotation_apply_denotation g'_def[abs_def] s'_def)
+  moreover have \<open>kraus_map s'\<close>
+    using apply_denotation is_cq_map_def s'_def by blast
+  ultimately show \<open>km_summable g' A\<close>
+    by (metis g'_def apply_denotation has_sum_coordinatewise is_cq_map_def km_summable_iff_sums_to_kraus_map
+        mem_Collect_eq)
+next
+  define g' where \<open>g' x = apply_denotation (g x)\<close> for x
+  then have km_g': \<open>kraus_map (g' x)\<close> for x
+    using apply_denotation is_cq_map_def by force
+  assume asm: \<open>km_summable g' A\<close>
+  then obtain s' where \<open>((\<lambda>x. g' x t) has_sum s' t) A\<close> and \<open>kraus_map s'\<close> for t
+    apply (subst (asm) km_summable_iff_sums_to_kraus_map[OF km_g'])
+    by fastforce
+  then have sum_s: \<open>(g' has_sum s') A\<close>
+    by (simp add: has_sum_coordinatewise)
+  then obtain s' where sum_s: \<open>(g' has_sum s') A\<close>
+    using summable_on_def by blast
+  then have \<open>is_cq_map qFst s'\<close>
+    apply (rule is_cq_map_has_sum[rotated 2])
+    using apply_denotation asm g'_def[abs_def] asm by auto
+  then obtain s where \<open>s' = apply_denotation s\<close>
+    using apply_denotation_cases by blast
+  with sum_s have \<open>(g' has_sum apply_denotation s) A\<close>
+    by simp
+  then have \<open>(g has_sum s) A\<close>
+    by (simp add: g'_def[abs_def] has_sum_denotation_apply_denotation)
+  then show \<open>g summable_on A\<close>
+    by (simp add: has_sum_imp_summable)
+qed
+
+
+lemma summable_on_denotation_transfer[transfer_rule]:
+  includes lifting_syntax
+  shows \<open>(((=) ===> cr_denotation) ===> (=) ===> (\<longleftrightarrow>)) (\<lambda>g A. km_summable g A) Infinite_Sum.summable_on\<close>
+  apply (simp add: summable_on_denotation_apply_denotation[abs_def])
+  by transfer_prover
+
 lemma
   assumes \<open>denotation_norm D \<le> 1\<close>
   shows denotation_while_bounded[iff]: \<open>denotation_norm (denotation_while e D) \<le> 1\<close>
     and denotation_while_has_sum: \<open>(denotation_while_n e D has_sum denotation_while e D) UNIV\<close>
 proof -
-(*   \<open>denotation_while_n e D n = (denotation_cases (\<lambda>m. if e m then D else 0))^n * (denotation_cases (\<lambda>m. if e m then 0 else 1))\<close> *)
   define W where \<open>W = denotation_while_n e D\<close>
   have rewrite_Wsum: \<open>(\<Sum>n\<le>M. W n) = (denotation_cases (\<lambda>m. if e m then D else 1))^M * (denotation_cases (\<lambda>m. if e m then 0 else 1))\<close> for M
-  proof (induction M)
-    case 0
-    show ?case
-      by (simp add: W_def denotation_while_n_def)
-  next
-    case (Suc M)
-    have \<open>(\<Sum>n\<le>Suc M. W n) = xxx\<close>
-      apply (simp add: )
-      by x
-    also have \<open>\<dots> = (denotation_cases (\<lambda>m. if e m then D else 1))^(Suc M) * (denotation_cases (\<lambda>m. if e m then 0 else 1))\<close>
-      by x
-    then show ?case
-      by -
-  qed
+    by (simp add: W_def denotation_while_n_sum)
   have finsum: \<open>(\<Sum>n\<in>F. km_bound (apply_denotation (W n))) \<le> id_cblinfun\<close> if \<open>finite F\<close> for F
   proof -
     define N where \<open>N = Max F\<close>
     have \<open>(\<Sum>n\<in>F. km_bound (apply_denotation (W n))) \<le> (\<Sum>n\<le>N. km_bound (apply_denotation (W n)))\<close>
       using that by (auto intro!: sum_mono2 simp: N_def)
-    have \<open>\<dots> = km_bound (\<Sum>n\<le>N. apply_denotation (W n))\<close>
-      by -
+    also have \<open>\<dots> = km_bound (\<Sum>n\<le>N. apply_denotation (W n))\<close>
+      apply (rule km_bound_sum[symmetric])
+      using apply_denotation is_cq_map_def by blast
     also have \<open>\<dots> = km_bound (apply_denotation (\<Sum>n\<le>N. W n))\<close>
-      by -
-    also have \<open>\<dots> = km_bound (apply_denotation XXXX)\<close>
-      by x
-    also have \<open>\<dots> = denotation_norm XXXX *\<^sub>C id_cblinfun\<close>
-      by -
-    also have \<open>\<dots> \<le> 1 *\<^sub>C id_cblinfun\<close>
-      by x
+      by (simp add: apply_denotation_sum)
+    also have \<open>\<dots> = km_bound (apply_denotation (denotation_cases (\<lambda>m. if e m then D else 1) ^ N * denotation_cases (\<lambda>m. if e m then 0 else 1)))\<close>
+      by (simp add: rewrite_Wsum)
+    also have \<open>\<dots> \<le> denotation_norm (denotation_cases (\<lambda>m. if e m then D else 1) ^ N * denotation_cases (\<lambda>m. if e m then 0 else 1)) *\<^sub>R id_cblinfun\<close>
+      by (simp add: denotation_norm.rep_eq km_bound_leq_km_norm_id)
+    also have \<open>\<dots> \<le> 1 *\<^sub>R id_cblinfun\<close> (is \<open>denotation_norm (?x^N * ?y) *\<^sub>R id_cblinfun \<le> _\<close>)
+      apply (rule scaleR_right_mono)
+      by (auto intro!: times_denotation_bounded[THEN order_trans] mult_le_one power_le_one
+          power_denotation_bounded[THEN order_trans] denotation_cases_bounded assms)
     also have \<open>\<dots> = id_cblinfun\<close>
       by simp
     finally show ?thesis
@@ -743,25 +1127,278 @@ proof -
   then have km_bound: \<open>km_bound (\<lambda>\<rho>. \<Sum>\<^sub>\<infinity>n. apply_denotation (W n) \<rho>) \<le> id_cblinfun\<close>
     apply (subst km_bound_infsum)
     using apply_denotation km_summable by (auto intro!: simp: is_cq_map_def)
-  have \<open>denotation_while_n e D summable_on UNIV\<close>
-    by -
-  then show \<open>(denotation_while_n e D has_sum denotation_while e D) UNIV\<close>
-    by (simp add: denotation_while_def)
-  have while_infsum: \<open>apply_denotation (denotation_while e D) \<rho> = (\<Sum>\<^sub>\<infinity>n. apply_denotation (W n) \<rho>)\<close> for \<rho>
-    by x
+  have \<open>W summable_on UNIV\<close>
+    by (simp add: summable_on_denotation_apply_denotation km_summable flip: W_def)
+  then show \<open>(W has_sum denotation_while e D) UNIV\<close>
+    by (simp add: denotation_while_def W_def)
+  then have \<open>((\<lambda>n. apply_denotation (W n) \<rho>) has_sum apply_denotation (denotation_while e D) \<rho>) UNIV\<close> for \<rho>
+    by (simp add: has_sum_denotation_apply_denotation has_sum_coordinatewise)
+  then have while_infsum: \<open>apply_denotation (denotation_while e D) \<rho> = (\<Sum>\<^sub>\<infinity>n. apply_denotation (W n) \<rho>)\<close> for \<rho>
+    by (metis infsumI)
   show \<open>denotation_norm (denotation_while e D) \<le> 1\<close>
     using norm_cblinfun_mono[OF _ km_bound]
     by (simp_all add: denotation_norm.rep_eq km_norm_def while_infsum[abs_def])
 qed
 
+lemma km_tensor_0_left[simp]: \<open>km_tensor (0 :: ('a ell2, 'b ell2) trace_class \<Rightarrow> ('c ell2, 'd ell2) trace_class) \<EE> = 0\<close>
+proof (cases \<open>km_tensor_exists (0 :: ('a ell2, 'b ell2) trace_class \<Rightarrow> ('c ell2, 'd ell2) trace_class) \<EE>\<close>)
+  case True
+  then show ?thesis
+    apply (rule_tac eq_from_separatingI2[OF separating_set_bounded_clinear_tc_tensor])
+    by (simp_all add: km_tensor_apply)
+next
+  case False
+  then show ?thesis
+    using km_tensor_invalid by blast
+qed
+
+lemma km_tensor_0_right[simp]: \<open>km_tensor \<EE> (0 :: ('a ell2, 'b ell2) trace_class \<Rightarrow> ('c ell2, 'd ell2) trace_class) = 0\<close>
+proof (cases \<open>km_tensor_exists \<EE> (0 :: ('a ell2, 'b ell2) trace_class \<Rightarrow> ('c ell2, 'd ell2) trace_class)\<close>)
+  case True
+  then show ?thesis
+    apply (rule_tac eq_from_separatingI2[OF separating_set_bounded_clinear_tc_tensor])
+    by (simp_all add: km_tensor_apply)
+next
+  case False
+  then show ?thesis
+    using km_tensor_invalid by blast
+qed
+
+
+lemma cq_id_qregister_pair:
+  assumes \<open>qcompatible Q R\<close>
+  shows \<open>cq_id \<lbrakk>Q,R\<rbrakk>\<^sub>q = cq_id Q o cq_id R\<close>
+  unfolding cq_id_def
+  apply (subst km_complete_measurement_ket_tensor[symmetric])
+  apply (subst km_apply_qregister_pair_tensor)
+  using assms by auto
+
+
+lemma cq_id_qregister_chain:
+  \<open>cq_id (qregister_chain Q R) = km_apply_qregister Q (cq_id R)\<close>
+  by (simp add: cq_id_def km_apply_qregister_chain)
+
+
+lemma cq_id_qregister_tensor: 
+  \<open>cq_id (qregister_tensor Q R) = km_tensor (cq_id Q) (cq_id R)\<close>
+proof -
+  wlog [iff]: \<open>qregister Q\<close> \<open>qregister R\<close>
+    using negation
+    by (auto simp: cq_id_invalid non_qregister)
+  show ?thesis
+    apply (rule_tac eq_from_separatingI2[OF separating_set_bounded_clinear_tc_tensor])
+      apply simp 
+     apply (simp add: km_tensor_kraus_map kraus_map_bounded_clinear) 
+    by (simp add: qregister_tensor_pair cq_id_qregister_pair cq_id_qregister_chain
+        km_apply_qregister_pair_tensor km_apply_qregister_qFst km_apply_qregister_qSnd km_tensor_apply
+        km_tensor_kraus_map_exists)
+qed
+
+lemma is_cq_map_qregister_tensor:
+  assumes \<open>is_cq_map Q \<EE>\<close>
+  assumes \<open>is_cq_map R \<FF>\<close>
+  shows \<open>is_cq_map (qregister_tensor Q R) (km_tensor \<EE> \<FF>)\<close>
+proof (intro is_cq_map_def[THEN iffD2] conjI)
+  from assms have [iff]: \<open>kraus_map \<EE>\<close>  \<open>kraus_map \<FF>\<close>
+    using is_cq_map_def by auto
+  then show \<open>kraus_map (km_tensor \<EE> \<FF>)\<close>
+    by (meson km_tensor_kraus_map)
+  have \<open>cq_id (qregister_tensor Q R) \<circ> km_tensor \<EE> \<FF> \<circ> cq_id (qregister_tensor Q R)
+    = km_tensor (cq_id Q) (cq_id R) o km_tensor \<EE> \<FF> o km_tensor (cq_id Q) (cq_id R)\<close>
+    by (simp add: cq_id_qregister_tensor)
+  also have \<open>\<dots> = km_tensor (cq_id Q o \<EE> o cq_id Q) (cq_id R o \<FF> o cq_id R)\<close>
+    by (simp add: km_tensor_compose_distrib km_tensor_kraus_map_exists kraus_map_comp)
+  also have \<open>\<dots> = km_tensor \<EE> \<FF>\<close>
+    by (metis assms(1,2) is_cq_map_def)
+  finally show \<open>cq_id (qregister_tensor Q R) \<circ> km_tensor \<EE> \<FF> \<circ> cq_id (qregister_tensor Q R) = km_tensor \<EE> \<FF>\<close>
+    by -
+qed
+
+(* TODO move TODO name *)
+lemma [iff]: \<open>iso_qregister \<lbrakk>qregister_id, empty_qregister\<rbrakk>\<^sub>q\<close>
+  by (metis iso_qregister_def' iso_qregister_id qcompatible_empty qregister_chain_is_qregister
+      qregister_chain_pair_Fst qregister_left_right_inverse)
+
+lemma one_dim_butterfly:
+  \<open>butterfly g h = (one_dim_iso g * cnj (one_dim_iso h)) *\<^sub>C 1\<close>
+  apply (rule cblinfun_eq_on_canonical_basis)
+  apply simp
+  by (smt (verit, del_insts) Groups.mult_ac(2) cblinfun.scaleC_left of_complex_def of_complex_inner_1
+      of_complex_inner_1' one_cblinfun_apply_one one_dim_apply_is_times_def one_dim_iso_def
+      one_dim_scaleC_1)
+
+
+lemma one_dim_tc_butterfly:
+  fixes g :: \<open>'a :: one_dim\<close> and h :: \<open>'b :: one_dim\<close>
+  shows \<open>tc_butterfly g h = (one_dim_iso g * cnj (one_dim_iso h)) *\<^sub>C 1\<close>
+proof -
+  have \<open>tc_butterfly g h = one_dim_iso (butterfly g h)\<close>
+  by (metis (mono_tags, lifting) from_trace_class_one_dim_iso one_dim_iso_inj one_dim_iso_is_of_complex
+      one_dim_iso_of_complex tc_butterfly.rep_eq)
+  also have \<open>\<dots> = (one_dim_iso g * cnj (one_dim_iso h)) *\<^sub>C 1\<close>
+    by (simp add: one_dim_butterfly)
+  finally show ?thesis
+    by -
+qed
+
+(* lemma one_dim_iso_tc_butterfly:
+  fixes g :: \<open>'a :: one_dim\<close> and h :: \<open>'b :: one_dim\<close>
+  shows \<open>one_dim_iso (tc_butterfly g h) = one_dim_iso (cnj (one_dim_iso g) * one_dim_iso h)\<close>
+proof -
+  have \<open>one_dim_iso (tc_butterfly g h) = one_dim_iso (one_dim_iso (tc_butterfly g h) :: 'b \<Rightarrow>\<^sub>C\<^sub>L 'a)\<close>
+    by auto
+  also have \<open>\<dots> = one_dim_iso (from_trace_class (tc_butterfly g h))\<close>
+    by simp
+  also have \<open>\<dots> = one_dim_iso (butterfly g h)\<close>
+    by (metis tc_butterfly.rep_eq)
+  also have \<open>\<dots> = one_dim_iso (cnj (one_dim_iso g) * one_dim_iso h)\<close>
+    by (simp add: one_dim_iso_tc_butterfly)
+  finally show ?thesis
+    by -
+qed
+ *)
+
+lemma one_dim_iso_of_real[simp]: \<open>one_dim_iso (of_real x) = of_real x\<close>
+  apply (simp add: of_real_def)
+  by (simp add: scaleR_scaleC del: of_complex_of_real_eq)
+
+lemma kf_one_dim_is_id[simp]:
+  fixes \<EE> :: \<open>('a::one_dim, 'a::one_dim, 'x) kraus_family\<close>
+  shows \<open>\<EE> =\<^sub>k\<^sub>r kf_norm \<EE> *\<^sub>R kf_id\<close>
+proof (rule kf_eq_weakI)
+  fix t :: \<open>('a, 'a) trace_class\<close>
+  have \<EE>1pos[iff]: \<open>\<EE> *\<^sub>k\<^sub>r 1 \<ge> 0\<close>
+    apply (rule kf_apply_pos)
+    by (metis one_cinner_one one_dim_iso_of_one one_dim_scaleC_1 tc_butterfly_pos trace_tc_butterfly
+          trace_tc_one_dim_iso)
+
+  have \<EE>t: \<open>\<EE> *\<^sub>k\<^sub>r t = trace_tc t *\<^sub>C (\<EE> *\<^sub>k\<^sub>r 1)\<close> if \<open>NO_MATCH 1 t\<close>for t
+    by (metis kf_apply_scaleC one_dim_scaleC_1 trace_tc_one_dim_iso)
+  have \<open>kf_bound \<EE> = norm (\<EE> *\<^sub>k\<^sub>r 1) *\<^sub>R id_cblinfun\<close>
+  proof (rule cblinfun_cinner_eqI)
+    fix h :: 'a
+    assume \<open>norm h = 1\<close>
+    have \<open>h \<bullet>\<^sub>C kf_bound \<EE> h = one_dim_iso h * cnj (one_dim_iso h) * one_dim_iso (\<EE> *\<^sub>k\<^sub>r 1)\<close>
+      apply (subst kf_bound_from_map)
+      by (simp add: \<EE>t cinner_scaleR_right cblinfun.scaleR_left cdot_square_norm one_dim_tc_butterfly)
+    also have 1: \<open>\<dots> = one_dim_iso (\<EE> *\<^sub>k\<^sub>r 1)\<close>
+      by (smt (verit, best) \<open>norm h = 1\<close> cinner_simps(5) cnorm_eq_1 id_apply more_arith_simps(6) mult.commute
+          one_dim_iso_def one_dim_iso_id one_dim_iso_is_of_complex one_dim_scaleC_1)
+    also have \<open>\<dots> = trace_tc (\<EE> *\<^sub>k\<^sub>r 1)\<close>
+      by simp
+    also have \<open>\<dots> = norm (\<EE> *\<^sub>k\<^sub>r 1)\<close>
+      apply (subst norm_tc_pos)
+      by (simp_all add: \<EE>1pos)
+    also have \<open>\<dots> = h \<bullet>\<^sub>C (norm (\<EE> *\<^sub>k\<^sub>r 1) *\<^sub>R id_cblinfun *\<^sub>V h)\<close>
+      by (metis \<open>norm h = 1\<close> cblinfun.scaleR_left cinner_commute cinner_scaleR_left cnorm_eq_1
+          complex_cnj_complex_of_real id_cblinfun.rep_eq mult.commute mult_cancel_right1)
+    finally show \<open>h \<bullet>\<^sub>C (kf_bound \<EE> *\<^sub>V h) = h \<bullet>\<^sub>C (norm (\<EE> *\<^sub>k\<^sub>r 1) *\<^sub>R id_cblinfun *\<^sub>V h)\<close>
+      by -
+  qed
+  then have \<open>kf_norm \<EE> = cmod (one_dim_iso (\<EE> *\<^sub>k\<^sub>r 1))\<close>
+    by (simp add: kf_norm_def)
+  then have norm: \<open>complex_of_real (kf_norm \<EE>) = one_dim_iso (\<EE> *\<^sub>k\<^sub>r 1)\<close>
+  using norm_tc_pos by fastforce
+
+  have \<open>(one_dim_iso (\<EE> *\<^sub>k\<^sub>r t) :: complex) = one_dim_iso t * one_dim_iso (\<EE> *\<^sub>k\<^sub>r 1)\<close>
+  by (metis (mono_tags, lifting) kf_apply_scaleC of_complex_one_dim_iso one_dim_iso_is_of_complex
+      one_dim_iso_scaleC one_dim_scaleC_1 scaleC_one_dim_is_times)
+  also have \<open>\<dots> = one_dim_iso t * complex_of_real (kf_norm \<EE>)\<close>
+    by (simp add: norm)
+  also have \<open>\<dots> = one_dim_iso (kf_norm \<EE> *\<^sub>R t)\<close>
+    by (simp add: scaleR_scaleC)
+  also have \<open>\<dots> = one_dim_iso (kf_norm \<EE> *\<^sub>R kf_id *\<^sub>k\<^sub>r t)\<close>
+    by (simp add: kf_scale_apply)
+  finally show \<open>\<EE> *\<^sub>k\<^sub>r t = kf_norm \<EE> *\<^sub>R kf_id *\<^sub>k\<^sub>r t\<close>
+    using one_dim_iso_inj by blast
+qed
+
+
+
+lemma kf_apply_qregister_scaleR:
+  shows \<open>kf_apply_qregister Q (r *\<^sub>R \<EE>) = r *\<^sub>R kf_apply_qregister Q \<EE>\<close>
+  apply (transfer' fixing: r Q)
+  by (force simp: apply_qregister_scaleR image_iff)
+
+lemma kf_apply_qregister_kf_id[simp]:
+  assumes \<open>qregister Q\<close>
+  shows \<open>kf_apply_qregister Q kf_id = kf_id\<close>
+  unfolding kf_id_def
+  apply (transfer' fixing: Q)
+  by (simp add: assms)
+
+lemma kf_apply_qregister_empty_qregister: 
+  \<open>kf_apply_qregister (empty_qregister :: ('a::{CARD_1,enum},'b) qregister) \<EE> =\<^sub>k\<^sub>r kf_norm \<EE> *\<^sub>R kf_id\<close>
+proof -
+  let ?e = \<open>empty_qregister :: ('a::{CARD_1,enum},'b) qregister\<close>
+  have \<open>kf_apply_qregister ?e \<EE> =\<^sub>k\<^sub>r kf_apply_qregister ?e (kf_norm \<EE> *\<^sub>R kf_id)\<close>
+    apply (rule kf_apply_qregister_cong_weak)
+    by (rule kf_one_dim_is_id)
+  also have \<open>\<dots> = kf_norm \<EE> *\<^sub>R kf_apply_qregister ?e kf_id\<close>
+    by (rule kf_apply_qregister_scaleR)
+  also have \<open>\<dots> = kf_norm \<EE> *\<^sub>R kf_id\<close>
+    by simp
+  finally show ?thesis
+    by -
+qed
+
+lemma km_apply_qregister_empty_qregister[simp]: 
+  assumes \<open>kraus_map \<EE>\<close>
+  shows \<open>km_apply_qregister empty_qregister \<EE> t = km_norm \<EE> *\<^sub>R t\<close>
+  using kf_apply_qregister_empty_qregister[of \<open>km_some_kraus_family \<EE>\<close>, where 'b='b]
+  using assms
+  by (simp add: kf_eq_weak_def kf_scale_apply[OF km_norm_geq0, abs_def]
+      flip: km_apply_qregister_kf_apply)
+
+
+lemma cq_id_empty_qregister[simp]: \<open>cq_id empty_qregister = id\<close>
+  by (auto intro!: ext simp add: cq_id_def)
+
+
+lemma is_cq_map_empty_qregister[simp]: \<open>is_cq_map empty_qregister \<EE> \<longleftrightarrow> kraus_map \<EE>\<close>
+  by (simp add: is_cq_map_def)
+
+lemma is_cq_map_qFst_chain:
+  assumes [iff]: \<open>is_cq_map Q \<EE>\<close>
+  assumes [iff]: \<open>kraus_map \<FF>\<close>
+  shows \<open>is_cq_map (qregister_chain qFst Q) (km_tensor \<EE> \<FF>)\<close>
+proof (intro is_cq_map_def[THEN iffD2] conjI)
+  from assms have [iff]: \<open>kraus_map \<EE>\<close>
+    using is_cq_map_def by auto
+  with assms show \<open>kraus_map (km_tensor \<EE> \<FF>)\<close>
+    by (meson km_tensor_kraus_map)
+  have \<open>cq_id (qregister_chain qFst Q) \<circ> km_tensor \<EE> \<FF> \<circ> cq_id (qregister_chain qFst Q)
+    = km_tensor (cq_id Q) id \<circ> km_tensor \<EE> \<FF> \<circ> km_tensor (cq_id Q) id\<close>
+    by (simp add: cq_id_qregister_chain km_apply_qregister_qFst)
+  also have \<open>\<dots> = km_tensor (cq_id Q o \<EE> o cq_id Q) \<FF>\<close>
+    by (simp add: km_tensor_kraus_map_exists kraus_map_comp flip: km_tensor_compose_distrib)
+  also have \<open>\<dots> = km_tensor \<EE> \<FF>\<close>
+    by (metis assms(1,2) is_cq_map_def)
+  finally show \<open>cq_id (qregister_chain qFst Q) \<circ> km_tensor \<EE> \<FF> \<circ> cq_id (qregister_chain qFst Q) = km_tensor \<EE> \<FF>\<close>
+    by -
+qed
+
+lemma is_cq_map_qFst[intro!]:
+  assumes \<open>is_cq_map qregister_id \<EE>\<close>
+  assumes \<open>kraus_map \<FF>\<close>
+  shows \<open>is_cq_map qFst (km_tensor \<EE> \<FF>)\<close>
+  using is_cq_map_qFst_chain[OF assms]
+  by simp
+
+lemma is_cq_map_complete_measurement[iff]: 
+  \<open>is_cq_map qregister_id km_complete_measurement_ket\<close>
+  by (simp add: is_cq_map_def cq_id_def comp_def)
 
 definition denotation_from_quantum :: \<open>(cl \<Rightarrow> (qu ell2, qu ell2) trace_class \<Rightarrow> (qu ell2, qu ell2) trace_class) \<Rightarrow> denotation\<close> where
-  \<open>denotation_from_quantum q = denotation_cases (\<lambda>c. Abs_denotation (km_tensor id (q c)))\<close>
+  \<open>denotation_from_quantum q = denotation_cases (\<lambda>c. Abs_denotation (km_tensor km_complete_measurement_ket (q c)))\<close>
 
 lemma denotation_from_quantum_bounded[iff]:
+  assumes \<open>\<And>c. kraus_map (q c)\<close>
   assumes \<open>\<And>c. km_norm (q c) \<le> 1\<close>
   shows \<open>denotation_norm (denotation_from_quantum q) \<le> 1\<close>
-  by x
+  unfolding denotation_from_quantum_def
+  apply (rule denotation_cases_bounded)
+  by (simp add: eq_onp_def is_cq_map_qFst assms denotation_norm.abs_eq km_norm_tensor)
 
 fun denotation_raw :: \<open>raw_program \<Rightarrow> denotation\<close> where
   denotation_raw_Skip: \<open>denotation_raw Skip = 1\<close>
@@ -778,8 +1415,15 @@ fun denotation_raw :: \<open>raw_program \<Rightarrow> denotation\<close> where
 | denotation_raw_LocalC: \<open>denotation_raw (LocalC F init c) = denotation_local_c F init (denotation_raw c)\<close>
 | denotation_raw_LocalQ: \<open>denotation_raw (LocalQ F init c) = denotation_local_q F init (denotation_raw c)\<close>
 
-lemma denotation_raw_bounded: \<open>denotation_bounded (denotation_raw p)\<close> if \<open>valid_oracle_program p\<close>
-    using that apply induction by auto
+lemma denotation_raw_bounded: \<open>denotation_norm (denotation_raw p) \<le> 1\<close> if \<open>valid_oracle_program p\<close>
+  using that apply induction
+  by (auto intro!: 
+      times_denotation_bounded[THEN order.trans, OF mult_le_one]
+      denotation_cases_bounded
+      denotation_from_quantum_bounded
+      denotation_local_q_bounded[THEN order.trans]
+      denotation_local_c_bounded[THEN order.trans])
+
 
 (* fun denotation_raw :: "raw_program \<Rightarrow> cq_map" where
   denotation_raw_Skip: \<open>denotation_raw Skip = cq_kf_id\<close>
@@ -796,36 +1440,29 @@ fun denotation_raw :: "raw_program \<Rightarrow> cq_operator \<Rightarrow> cq_op
 
 lift_definition denotation :: "program \<Rightarrow> denotation" is denotation_raw.
 
-lemma denotation_bounded[iff]: \<open>denotation_bounded (denotation p)\<close>
+lemma denotation_bounded[iff]: \<open>denotation_norm (denotation p) \<le> 1\<close>
   apply transfer
   by (auto intro!: denotation_raw_bounded simp: valid_program_def)
 
 lemma denotation_sample: \<open>denotation (sample x e) = denotation_sample (\<lambda>m. map_distr (\<lambda>xa. Classical_Registers.setter x xa m) (e m))\<close>
-  apply (transfer' fixing: x e)
-  by simp
+  by (simp add: denotation.rep_eq sample.rep_eq)
 
 
-
-lemma kf_norm_sample_prob: \<open>kf_norm (kraus_map_sample (prob \<mu>) :: ('a::{chilbert_space,not_singleton},'a,'x) kraus_family) = weight \<mu>\<close>
-  apply (subst kraus_map_sample_norm[of \<open>prob \<mu>\<close>])
+lemma kf_norm_sample_prob: \<open>kf_norm (kf_sample (prob \<mu>) :: ('a::{chilbert_space,not_singleton},'a,'x) kraus_family) = weight \<mu>\<close>
+  apply (subst kf_sample_norm[of \<open>prob \<mu>\<close>])
   by (auto intro!: prob_summable simp: Prob.rep_eq)
 
-lemma kraus_map_sample_point_distr': \<open>kf_remove_0 (kraus_map_sample (prob (point_distr x))) 
-                                        = kf_remove_0 (kf_map_outcome_inj (\<lambda>_. x) kf_id)\<close>
+lemma kraus_map_sample_point_distr': \<open>(kf_sample (prob (point_distr x))) 
+                                        = (kf_map_inj (\<lambda>_. x) kf_id)\<close>
   apply (rule Rep_kraus_family_inject[THEN iffD1])
   by (auto intro!: prob_summable
-      simp: kraus_map_sample.rep_eq kf_map_outcome_inj.rep_eq kf_id_def
-      kf_of_op.rep_eq kf_remove_0.rep_eq image_iff
+      simp: kf_sample.rep_eq kf_map_inj.rep_eq kf_id_def
+      kf_of_op.rep_eq image_iff
       simp del: kf_of_op_id)
 
-lemma kraus_map_sample_point_distr: \<open>kraus_equivalent' (kraus_map_sample (prob (point_distr x))) (kf_map_outcome_inj (\<lambda>_. x) kf_id)\<close>
-  using kraus_map_sample_point_distr'[of x] kf_remove_0_equivalent'
-    kraus_equivalent'_sym kraus_equivalent'_trans
-  by metis
-
-lemma cq_map_sample_point_distr: \<open>cq_map_equiv (cq_map_sample (\<lambda>x. point_distr (f x))) (cq_map_classical f)\<close>
+(* lemma cq_map_sample_point_distr: \<open>cq_map_equiv (cq_map_sample (\<lambda>x. point_distr (f x))) (cq_map_classical f)\<close>
   apply (transfer' fixing: )
-  by (auto intro!: kraus_map_sample_point_distr simp: kf_norm_sample_prob)
+  by (auto intro!: kraus_map_sample_point_distr simp: kf_norm_sample_prob) *)
 
 lemma denotation_assign_sample: \<open>denotation (assign x e) = denotation_sample (\<lambda>m. point_distr (Classical_Registers.setter x (e m) m))\<close>
   by (simp add: assign_def denotation_sample)
